Begin Refinement

Uppaal_Networks/UPPAAL_Asm_AbsInt_Refine.thy
@@ -10,16 +10,39 @@ proof standard
   show "snd ` {s \<in> states. fst s = pc} \<subseteq> states_at states pc" by standard (auto simp: states_at.intros)
 qed
 
-datatype 'a rbt_state_map = RBT_SM "(addr * 'a) rbt"
+type_synonym 'a rbt_state_map = "(addr * 'a) rbt"
 
 fun def :: "'a \<Rightarrow> 'a option \<Rightarrow> 'a" where
   "def _ (Some v) = v" |
   "def d _ = d"
 
-definition RBT_SM :: "(addr * 'a) rbt \<Rightarrow> ('a::bot) state_map" where
-  "RBT_SM tree = SM (\<lambda>pc. def \<bottom> (Lookup2.lookup tree pc))"
+fun rbt_lookup :: "('a::bot) rbt_state_map \<Rightarrow> addr \<Rightarrow> 'a" where
+  "rbt_lookup tree pc = def \<bottom> (Lookup2.lookup tree pc)"
 
-code_datatype RBT_SM
+definition RBT_SM :: "(addr * 'a) rbt \<Rightarrow> ('a::bot) state_map" where
+  "RBT_SM tree = SM (rbt_lookup tree)"
+
+
+(*code_datatype RBT_SM*)
+
+lemma assumes "rbt t" "sorted1(inorder t)" shows "Lookup2.lookup (update k v t) k = Some v"
+proof -
+  from assms have "Lookup2.lookup (update k v t) = Lookup2.lookup t(k \<mapsto> v)" by (simp add: M.map_update M.invar_def)
+  thus ?thesis by simp
+qed
+
+fun merge_single :: "('a::sup) state_map \<Rightarrow> addr \<Rightarrow> 'a \<Rightarrow> 'a state_map" where
+  "merge_single (SM m) pc x = SM (\<lambda>npc. if npc = pc then x \<squnion> m npc else m npc)"
+
+fun rbt_merge_single :: "('a::{semilattice_sup, bot, linorder}) rbt_state_map \<Rightarrow> addr \<Rightarrow> 'a \<Rightarrow> 'a rbt_state_map" where
+  "rbt_merge_single tree pc x = update pc (x \<squnion> (rbt_lookup tree pc)) tree"
+
+lemma[code]: "merge_single (RBT_SM tree) pc x = RBT_SM (rbt_merge_single tree pc x)"
+proof(rule lookup_eq)
+  obtain m where func: "RBT_SM tree = SM m" using state_map_single_constructor by blast
+  have "(if k = pc then x \<squnion> m k else m k) = lookup (RBT_SM (rbt_merge_single tree pc x)) k" for k sorry
+  then show "lookup (merge_single (RBT_SM tree) pc x) k = lookup (RBT_SM (rbt_merge_single tree pc x)) k" for k by (simp add: func)
+qed
 
 lemma deepen_RBT_SM[code]:
   "deepen (set states) = propagate (RBT_SM empty) (set states)" sorry
