Uppaal_Networks/UPPAAL_Asm_AbsInt_MapRefine.thy
@@ -1,0 +1,42 @@
+theory UPPAAL_Asm_AbsInt_MapRefine
+imports                   
+  "HOL-Library.RBT_Mapping"
+  UPPAAL_Asm_AbsInt
+begin
+
+type_synonym 'a r_state_map = "(addr, 'a) mapping"
+
+fun r_lookup :: "('a::bot) r_state_map \<Rightarrow> addr \<Rightarrow> 'a" where
+  "r_lookup m = Mapping.lookup_default \<bottom> m"
+
+definition RSM :: "('a::bot) r_state_map \<Rightarrow> 'a state_map" where
+  "RSM m = SM (r_lookup m)"
+
+code_datatype RSM
+
+lemma[code]: "lookup (RSM m) = r_lookup m"
+  by (simp add: RSM_def)
+
+fun merge_single :: "('a::sup) state_map \<Rightarrow> addr \<Rightarrow> 'a \<Rightarrow> 'a state_map" where
+  "merge_single (SM m) pc x = SM (\<lambda>npc. if npc = pc then x \<squnion> m npc else m npc)"
+
+fun r_merge_single :: "('a::{semilattice_sup, bot, linorder}) r_state_map \<Rightarrow> addr \<Rightarrow> 'a \<Rightarrow> 'a r_state_map" where
+  "r_merge_single tree pc x = Mapping.update pc (x \<squnion> (r_lookup tree pc)) tree"
+
+lemma "pc \<noteq> ppc \<Longrightarrow> lookup (RSM (r_merge_single m pc x)) k = lookup (RSM m) k" sorry
+
+lemma[code]: "merge_single (RSM m) pc x = RSM (r_merge_single m pc x)"
+proof(rule lookup_eq)
+  obtain mm where func: "RSM m = SM mm" using state_map_single_constructor by blast
+  have "(if k = pc then x \<squnion> mm k else mm k) = lookup (RSM (r_merge_single m pc x)) k" for k
+  proof(cases "k = pc")
+    case True
+    then show ?thesis sorry
+  next
+    case False
+    then show ?thesis sorry
+  qed
+  thus "lookup (merge_single (RSM m) pc x) k = lookup (RSM (r_merge_single m pc x)) k" for k by (simp add: func)
+qed
+
+end
